MirrorCharge!/src/MirrorCharge/Java/Reify.v
@@ -57,6 +57,15 @@ Reify Declare Syntax reify_imp_typ :=
 
 Reify Declare Typed Table term_table : BinNums.positive => reify_imp_typ.
 
+Check term_table.
+
+Locate exprD.
+
+Require Import MirrorCore.ExprI.
+
+Check @exprD.
+Print Expr.
+Print RType.
 Let Ext x := @ExprCore.Inj typ func (inl (inl (inl (inl (inl (inl (inl (inl x)))))))).
 
 Reify Declare Syntax reify_imp :=
@@ -68,7 +77,7 @@ Reify Declare Syntax reify_imp :=
     	 (@Patterns.CTypedTable _ _ _ term_table Ext) :: nil))
   }.
 
-Definition stack_get (x : var) (s : stack) := s x.
+Definition stack_get (x : Lang.var) (s : stack) := s x.
 
 Notation "'ap_eq' '[' x ',' y ']'" :=
 	 (ap (T := Fun stack) (ap (T := Fun stack) (pure (T := Fun stack) (@eq val)) x) y).
@@ -104,7 +113,7 @@ Reify Pattern patterns_java_typ += (@RImpl (?0) (?1)) => (fun (a b : function re
 
 Reify Pattern patterns_java_typ += (!! asn)  => tyAsn.
 Reify Pattern patterns_java_typ += (!! sasn) => tySasn.
-Reify Pattern patterns_java_typ += (!! (@vlogic var val)) => tyPure.
+Reify Pattern patterns_java_typ += (!! (@vlogic Lang.var val)) => tyPure.
 Reify Pattern patterns_java_typ += (!! Prop) => tyProp.
 Reify Pattern patterns_java_typ += (!! spec) => tySpec.
 
@@ -113,23 +122,23 @@ Reify Pattern patterns_java_typ += (!! (@list String.string)) => tyVarList.
 Reify Pattern patterns_java_typ += (!! (@list field)) => tyFields.
 Reify Pattern patterns_java_typ += (!! (@list (@Open.expr (Lang.var) val))) => tyVarList.
 Reify Pattern patterns_java_typ += (!! (@list (Lang.var * @Open.expr (Lang.var) val))) => tySubstList.
-Reify Pattern patterns_java_typ += (!! (@substlist var val)) => tySubstList.
+Reify Pattern patterns_java_typ += (!! (@substlist Lang.var val)) => tySubstList.
 Reify Pattern patterns_java_typ += (!! @list @ ?0) => (fun x : function reify_imp_typ => tyList x).
 Reify Pattern patterns_java_typ += (!! nat) => tyNat.
 Reify Pattern patterns_java_typ += (!! val) => tyVal.
 Reify Pattern patterns_java_typ += (!! bool) => tyBool.
-Reify Pattern patterns_java_typ += (!! field) => tyField.
-Reify Pattern patterns_java_typ += (!! class) => tyClass.
-Reify Pattern patterns_java_typ += (!! @Open.open var val asn) => tySasn.
-Reify Pattern patterns_java_typ += (!! @Open.open var val Prop) => tyPure.
-Reify Pattern patterns_java_typ += (!! var) => tyVar.
+Reify Pattern patterns_java_typ += (!! field) => tyString.
+Reify Pattern patterns_java_typ += (!! class) => tyString.
+Reify Pattern patterns_java_typ += (!! @Open.open Lang.var val asn) => tySasn.
+Reify Pattern patterns_java_typ += (!! @Open.open Lang.var val Prop) => tyPure.
+Reify Pattern patterns_java_typ += (!! Lang.var) => tyString.
 Reify Pattern patterns_java_typ += (!! String.string) => tyString.
 Reify Pattern patterns_java_typ += (!! Program) => tyProg.
 Reify Pattern patterns_java_typ += (!! stack) => tyStack.
-Reify Pattern patterns_java_typ += (!! @Stack.stack var val) => tyStack.
+Reify Pattern patterns_java_typ += (!! @Stack.stack Lang.var val) => tyStack.
 Reify Pattern patterns_java_typ += (!! cmd) => tyCmd.
 Reify Pattern patterns_java_typ += (!! dexpr) => tyExpr.
-Reify Pattern patterns_java_typ += (!! (@Open.expr var val)) => tyExpr.
+Reify Pattern patterns_java_typ += (!! (@Open.expr Lang.var val)) => tyExpr.
 Reify Pattern patterns_java_typ += (!! @Subst.subst (String.string) val) => tySubst.
 
 Reify Pattern patterns_java_typ += (!! Fun @ ?0 @ ?1) => (fun (a b : function reify_imp_typ) => tyArr a b).
@@ -202,8 +211,8 @@ Reify Pattern patterns_java += (!! pointsto) => (fPointsto).
 Reify Pattern patterns_java += (!! prog_eq) => (fProgEq).
 Reify Pattern patterns_java += (!! typeof) => (fTypeOf).
 
-Reify Pattern patterns_java += (!! (@substl_trunc var val _)) => (fTruncSubst (func := expr typ func) (typ := typ)).
-Reify Pattern patterns_java += (!! (@substl var val _)) => (fSubst (func := expr typ func) (typ := typ)).
+Reify Pattern patterns_java += (!! (@substl_trunc Lang.var val _)) => (fTruncSubst (func := expr typ func) (typ := typ)).
+Reify Pattern patterns_java += (!! (@substl Lang.var val _)) => (fSubst (func := expr typ func) (typ := typ)).
 
 Reify Pattern patterns_java += (!! @nil @ ?0) => (fun (x : function reify_imp_typ) => (fNil (func := expr typ func) x)).
 Reify Pattern patterns_java += (!! @cons @ ?0) => (fun (x : function reify_imp_typ) => (fCons (func := expr typ func) x)).
@@ -212,8 +221,8 @@ Reify Pattern patterns_java += (!! @zip @ ?0 @ ?1) => (fun (x y : function reify
 Reify Pattern patterns_java += (!! @map @ ?0 @ ?1) => (fun (x y : function reify_imp_typ) => (fMap (func := expr typ func) x y)).
 Reify Pattern patterns_java += (!! @fold_right @ ?0 @ ?1) => (fun (x y : function reify_imp_typ) => (fFold (func := expr typ func) x y)).
 
-Reify Pattern patterns_java += (!! (@apply_subst var val) @ ?0) => (fun (x : function reify_imp_typ) => fApplySubst (func := expr typ func) x).
-Reify Pattern patterns_java += (!! @subst1 var val _) => (fSingleSubst (func := expr typ func)).
+Reify Pattern patterns_java += (!! (@apply_subst Lang.var val) @ ?0) => (fun (x : function reify_imp_typ) => fApplySubst (func := expr typ func) x).
+Reify Pattern patterns_java += (!! @subst1 Lang.var val _) => (fSingleSubst (func := expr typ func)).
 Reify Pattern patterns_java += (!! @field_lookup) => (fFieldLookup).
 (** Applicative **)
 Reify Pattern patterns_java += (!! @Applicative.ap @ !! (Fun stack) @ # @ ?0 @ ?1) => (fun (x y : function reify_imp_typ) => fAp (func := expr typ func) x y).
@@ -237,7 +246,7 @@ Goal (forall (Pr : Program) (C : class) (v : val) (fields : list field), True).
   reify_imp (field_lookup).
   reify_imp (field_lookup Pr C fields).
 
-  pose ((fun (_ : @Stack.stack var val) => null) : @Open.expr var val) as e2.
+  pose ((fun (_ : @Stack.stack Lang.var val) => null) : @Open.expr Lang.var val) as e2.
   pose ((fun (_ : stack) => null) : stack -> val) as e3.
 
 
@@ -263,7 +272,7 @@ Goal (forall (Pr : Program) (C : class) (v : val) (fields : list field), True).
   reify_imp (forall x : nat, x = x).
   reify_imp (exists x : nat, x = x).
   reify_imp (@map nat nat).
-  reify_imp (@subst1 var val _).
+  reify_imp (@subst1 Lang.var val _).
   reify_imp (cseq cskip cskip).
   
   reify_imp (ILogic.lentails True True).
@@ -295,375 +304,3 @@ Ltac reify_aux e n :=
   reify_expr reify_imp k
              [ (fun (y : @mk_dvar_map _ _ _ _ term_table elem_ctor) => True) ]
              [ e ].
-
-Definition mkPointstoVar x f e : expr typ func :=
-   mkAp tyVal tyAsn 
-        (mkAp tyField (tyArr tyVal tyAsn)
-              (mkAp tyVal (tyArr tyField (tyArr tyVal tyAsn))
-                    (mkConst (tyArr tyVal (tyArr tyField (tyArr tyVal tyAsn))) 
-                             fPointsto)
-                    (App fStackGet (mkVar x)))
-              (mkConst tyField (mkField f)))
-        e.
-
-Require Import MirrorCore.RTac.RTac.
-Require Import MirrorCore.Subst.FMapSubst.
-Require Import Coq.PArith.BinPos.
-
-Definition goalD_aux tus tvs goal (us : HList.hlist typD tus) (vs : HList.hlist typD tvs) :=
-  match goalD tus tvs goal with
-    | Some e => Some (e us vs)
-    | None => None
-  end.
-    
-Ltac cbv_denote e :=
-          eval cbv [
-          
-          goalD_aux
-          
-		  (* ExprD' *)
-          exprD' funcAs  typeof_sym typeof_func type_cast type_cast_typ
-          exprD'_simul func_simul
-          ExprD.Expr_expr
-          ExprDsimul.ExprDenote.exprD'
-          (* RSym *)
-          
-          SymSum.RSym_sum Rcast Relim Rsym eq_sym symD RSym_env
-          Rcast_val eq_rect_r eq_rect Datatypes.id
-          
-          (* Monad *)
-          
-          Monad.bind Monad.ret
-          
-          OptionMonad.Monad_option
-          
-          (* HList *)
-          
-          HList.hlist_hd HList.hlist_tl
-          
-          (* TypesI *)
-          
-          TypesI.typD 
-          typ2_match typ2 typ2_cast
-          typ0_match typ0 typ0_cast
-          (* ExprI *)
-          
-          MirrorCore.VariablesI.Var ExprVariables.ExprVar_expr
-          MirrorCore.VariablesI.UVar
-          MirrorCore.Lambda.ExprVariables.ExprUVar_expr
-          ExprI.exprT_Inj ExprI.exprT_UseV ExprI.exprT_UseU
-          exprT_App ExprI.exprT OpenT
-          nth_error_get_hlist_nth
-          
-          exprT_GetVAs exprT_GetUAs
-          
-          (* ILogicFunc*)
-          
-          ILogicFunc.mkEntails ILogicFunc.mkTrue ILogicFunc.mkFalse 
-          ILogicFunc.mkAnd ILogicFunc.mkOr ILogicFunc.mkImpl
-          ILogicFunc.mkExists ILogicFunc.mkForall
-          
-          ILogicFunc.fEntails ILogicFunc.fTrue ILogicFunc.fFalse ILogicFunc.fAnd 
-          ILogicFunc.fOr ILogicFunc.fImpl ILogicFunc.fExists ILogicFunc.fForall
-          ILogicFuncSumL ILogicFuncSumR ILogicFuncExpr
-          ILogicFunc.RSym_ilfunc 
-          MirrorCharge.ModularFunc.ILogicFunc.ILogicFuncInst
-          
-          ILogicFunc.funcD ILogicFunc.typ2_cast_quant ILogicFunc.typ2_cast_bin
-          
-          (* BILogicFunc *)
-          
-          BILogicFunc.mkEmp BILogicFunc.mkStar BILogicFunc.mkWand
-          
-          BILogicFunc.fEmp BILogicFunc.fStar BILogicFunc.fWand
-          
-          BILogicFuncSumL BILogicFuncSumR BILogicFuncExpr
-          BILogicFunc.RSym_bilfunc BILogicFunc.BILogicFuncInst
-          
-          BILogicFunc.funcD BILogicFunc.typ2_cast_bin
-          
-          BILogicFunc.typeof_bilfunc
-          
-          (* LaterFunc *)
-          
-          LaterFunc.mkLater
-          
-          LaterFunc.fLater
-          
-          LaterFunc.LaterFuncSumL LaterFunc.LaterFuncSumR LaterFunc.LaterFuncExpr          
-          LaterFunc.RSym_later_func LaterFunc.LaterFuncInst
-          
-          LaterFunc.funcD LaterFunc.typ2_cast'
-          
-          LaterFunc.typeof_later_func
-          
-          (* EmbedFunc *)
-          
-          EmbedFunc.mkEmbed
-          
-          EmbedFunc.fEmbed
-          
-          EmbedFunc.EmbedFuncSumL EmbedFunc.EmbedFuncSumR EmbedFuncExpr
-          EmbedFunc.RSym_embed_func EmbedFunc.EmbedFuncInst
-          
-          EmbedFunc.funcD EmbedFunc.typ2_cast_bin
-          
-
-          EmbedFunc.typeof_embed_func
-          
-          (* BaseFunc *)
-          
-          BaseFunc.BaseFuncSumL BaseFunc.BaseFuncSumR BaseFunc.BaseFuncExpr
-          
-          BaseFunc.BaseFuncInst
-          BaseFunc.mkNat BaseFunc.mkString BaseFunc.mkBool
-          BaseFunc.mkEq BaseFunc.mkPair
-          
-          BaseFunc.fNat BaseFunc.fString BaseFunc.fBool
-          BaseFunc.fEq BaseFunc.fPair
-          
-          BaseFunc.RSym_BaseFunc
-          
-          BaseFunc.typeof_base_func BaseFunc.base_func_eq BaseFunc.base_func_symD
-          BaseFunc.RelDec_base_func
-          
-          (* ListFunc *)
-          
-          ListFunc.ListFuncSumL ListFunc.ListFuncSumR ListFunc.ListFuncExpr
-          
-          ListFunc.ListFuncInst
-          ListFunc.mkNil ListFunc.mkCons ListFunc.mkLength 
-          ListFunc.mkZip ListFunc.mkMap ListFunc.mkFold
-          
-          ListFunc.fNil ListFunc.fCons ListFunc.fLength
-          ListFunc.fZip ListFunc.fMap ListFunc.fFold
-          
-          ListFunc.typeof_list_func ListFunc.list_func_eq ListFunc.list_func_symD
-          ListFunc.RelDec_list_func
-          
-		  (* OpenFunc *)
-		  
-		  OpenFunc.mkConst OpenFunc.mkAp OpenFunc.mkVar OpenFunc.mkNull OpenFunc.mkStackGet
-		  OpenFunc.mkStackSet OpenFunc.mkApplySubst OpenFunc.mkSingleSubst OpenFunc.mkSubst
-		  OpenFunc.mkTruncSubst
-		    
-		  OpenFunc.fConst OpenFunc.fAp OpenFunc.fVar OpenFunc.fNull OpenFunc.fStackGet
-		  OpenFunc.fApplySubst OpenFunc.fSingleSubst OpenFunc.fSubst OpenFunc.fTruncSubst
-		  
-		  OpenFunc.OpenFuncSumL OpenFunc.OpenFuncSumR OpenFunc.OpenFuncExpr
-		  OpenFunc.OpenFuncInst
-		  
-		  OpenFunc.typeof_open_func OpenFunc.RSym_OpenFunc
-		  OpenFunc.typ2_cast_bin OpenFunc.typ3_cast_bin
-		  OpenFunc.RelDec_open_func
-		  
-		  RSym_OpenFunc_obligation_1
-
-          (* BaseType *)
-          
-          BaseType.tyPair BaseType.tyNat BaseType.tyString BaseType.tyBool
-          BaseType.btPair BaseType.btNat BaseType.btBool BaseType.btString
-          
-          (* ListType *)
-          
-          ListType.tyList ListType.btList
-          
-          (* SubstType *)
-          
-          SubstType.tyVar SubstType.tyVal SubstType.tySubst
-          SubstType.stSubst
-          
-          (* JavaType *)
-         
-          Typ2_Fun Typ0_Prop RType_typ typD
-          should_not_be_necessary should_also_not_be_necessary
-         
-          JavaType.BaseType_typ JavaType.BaseTypeD_typ JavaType.ListType_typ
-          JavaType.ListTypeD_typ JavaType.bilops JavaType.ilops
-          JavaType.eops JavaType.lops
-          
-       (*   JavaType.typD *)
-		 (* JavaFunc *)
-          
-          ilops is_pure func RSym_JavaFunc typeof_java_func java_func_eq
-          java_func_symD RelDec_java_func
-                   
-          RSym_ilfunc RSym_open_func RSym_OpenFunc RSym_ListFunc
-          JavaFunc.RSym_bilfunc JavaFunc.RSym_embed_func JavaFunc.RSym_later_func
-          JavaFunc.RSym_ilfunc
-          JavaFunc.Expr_expr
-          mkPointstoVar
-          
-          JavaFunc.mkField JavaFunc.mkClass JavaFunc.mkVal JavaFunc.mkVarList
-          JavaFunc.mkProg JavaFunc.mkCmd JavaFunc.mkDExpr JavaFunc.mkFields
-          JavaFunc.fMethodSpec JavaFunc.fProgEq JavaFunc.fTriple JavaFunc.fTypeOf
-          JavaFunc.fFieldLookup JavaFunc.fPointsto JavaFunc.mkNull
-          JavaFunc.fPlus JavaFunc.fMinus JavaFunc.fTimes JavaFunc.fAnd
-          JavaFunc.fOr JavaFunc.fNot JavaFunc.fLt JavaFunc.fValEq
-          JavaFunc.mkTriple JavaFunc.mkFieldLookup JavaFunc.mkTypeOf
-          JavaFunc.mkProgEq JavaFunc.mkExprList JavaFunc.evalDExpr
-          
-          (* Applicative *)
-  (*        
-          ExtLib.Structures.Applicative.ap ExtLib.Structures.Applicative.pure
- 	      Applicative_Fun
-          
-          Charge.Logics.Pure.pure
-    *)      
-          SubstType_typ
-          
-          goalD propD exprD'_typ0 exprD split_env
-          
-          amap_substD
-          substD
-          SUBST.raw_substD
-          UVarMap.MAP.fold
-          FMapPositive.PositiveMap.fold
-          FMapPositive.PositiveMap.xfoldi
-          FMapPositive.append
-          UVarMap.MAP.from_key
-          pred
-          plus
-          Pos.to_nat
-          Pos.iter_op
-          app
-          HList.hlist_app
-          Quant._foralls
-          Quant._exists
-          ] in e.
-          Check app.
-
-Set Printing Depth 200.
-
-Ltac reify := 
-  let name := fresh "e" in
-  match goal with 
-  | |- ?P => reify_aux P name;
-	  let t := eval vm_compute in (typeof_expr nil nil name) in
-	  let e := eval unfold name in name in
-	  match t with
-	  | Some ?t =>  
-		  let e' := cbv_denote e t in
-		  match e' with
-		    | Some ?r => 
-		      let r' := constr:(r HList.Hnil HList.Hnil) in 
-		      	replace P with r' by exact eq_refl; clear name
-		    | _ => idtac e'
-		  end
-      | _ => idtac 1
-	  end
-   end.
-
-Definition run_tac tac goal :=
-  runOnGoals tac nil nil 0 0 (CTop nil nil) 
-    (ctx_empty (typ := typ) (expr := expr typ func)) goal.
-
-Lemma run_rtac_More tac s goal P e e'
-  (H : exprD nil nil e tyProp = Some P)
-  (Hres : run_tac tac (GGoal e) = More_ s goal) 
-  (Heval : goalD_aux nil nil goal HList.Hnil HList.Hnil = Some e')
-  (Hsound : rtac_sound tac) :
-  e' -> P.
-Proof.
-  intros He'.
-  unfold run_tac in Hres.
-  unfold rtac_sound in Hsound.
-  assert (WellFormed_Goal nil nil (GGoal (typ := typ) e)) as H1 by constructor.
-  assert (WellFormed_ctx_subst (TopSubst (expr typ func) nil (@nil typ))) as H2 by constructor.
-  specialize (Hsound _ _ _ _ Hres H1 H2).
-  destruct Hsound as [Hwfs [Hwfg Hsound]].
-  simpl in Hsound.
-  unfold propD, exprD'_typ0 in Hsound.
-  unfold exprD in H. simpl in H. 
-  
-  Require Import ExtLib.Tactics.
-  simpl in Hsound.
-  forward; inv_all; subst; destruct Hsound as [Hsubst2 Hsound].
-  inversion Hsubst2; subst.
-  specialize (Hsound HList.Hnil HList.Hnil).
-  simpl in Hsound.
-  inv_all; subst.
-  inversion Hwfs; subst.
-  simpl in H3; inv_all; subst.
-  apply Hsound.
-  unfold goalD_aux in Heval. forward; inv_all; subst.
-  assumption.
-Qed.
-
-Lemma run_rtac_Solved tac s P e
-  (H : exprD nil nil e tyProp = Some P)
-  (Hres : run_tac tac (GGoal e) = Solved s)
-  (Hsound : rtac_sound tac) :
-  P.
-Proof.
-  unfold run_tac in Hres.
-  unfold rtac_sound in Hsound.
-  assert (WellFormed_Goal nil nil (GGoal (typ := typ) e)) as H1 by constructor.
-  assert (WellFormed_ctx_subst (TopSubst (expr typ func) nil (@nil typ))) as H2 by constructor.
-  specialize (Hsound _ _ _ _ Hres H1 H2).
-  destruct Hsound as [Hwfs Hsound].
-  simpl in Hsound.
-  unfold propD, exprD'_typ0 in Hsound.
-  unfold exprD in H. simpl in H. 
-
-  simpl in Hsound.
-  forward; inv_all; subst; destruct Hsound as [Hsubst2 Hsound].
-  inversion Hsubst2; subst.
-  specialize (Hsound HList.Hnil HList.Hnil).
-  simpl in Hsound.
-  inv_all; subst.
-  inversion Hwfs; subst.
-  simpl in H3; inv_all; subst.
-  apply Hsound.
-Qed.
-
-Ltac run_rtac tac_sound :=
-  match type of tac_sound with
-    | rtac_sound ?tac =>
-	  let name := fresh "e" in
-	  match goal with
-	    | |- ?P => 
-	      reify_aux P name;
-	      let t := eval vm_compute in (typeof_expr nil nil name) in
-	      let goal := eval unfold name in name in
-	      match t with
-	        | Some ?t =>
-	          let goal_result := constr:(run_tac tac (GGoal goal)) in 
-	          let result := eval vm_compute in goal_result in 
-	          match result with
-	            | More_ ?s ?g =>
-	              let Q := cbv_denote (goalD_aux nil nil g HList.Hnil HList.Hnil) in
-	              match Q with
-	                | Some ?Q' => 
-	                  cut (Q' HList.Hnil HList.Hnil); [
-		              let P := cbv_denote (exprD nil nil goal tyProp) in 
-		              let H1 := fresh "H" in
-		              let H2 := fresh "H" in
-		              let H3 := fresh "H" in     
-		              let H4 := fresh "H" in      
-		              pose (H1 := @eq_refl (option Prop) P <: 
-		              	exprD nil nil goal tyProp = P);
-		              pose (H2 := @eq_refl (Result (CTop nil nil)) result <: 
-		              	run_tac tac (GGoal goal) = result);
-		              pose (H3 := @eq_refl (option (exprT nil nil Prop)) Q <:
-		              	goalD_aux nil nil g HList.Hnil HList.Hnil = Q);
-		              exact (@run_rtac_More tac _ _ _ _ _ H1 H2 H3 tac_sound) |]
-		            | None => idtac "Unable to find a denotation for" Q
-		          end
-	            | Solved ?s =>
-	              let P := cbv_denote (exprD nil nil goal tyProp) in
-	              let H1 := fresh "H" in
-	              pose (H1 := @eq_refl (option Prop) P <:
-	                exprD nil nil goal tyProp = P);
-		          pose (H2 := @eq_refl (Result (CTop nil nil)) result <: 
-		            run_tac tac (GGoal goal) = result);
-	              exact (@run_rtac_Solved tac _ _ _ H1 H2 tac_sound)
-	            | Fail => idtac "Tactic" tac "failed."
-	            | _ => idtac "Error: run_rtac could not resolve the result from the tactic :" result
-	          end
-	        | None => idtac "expression " goal "is ill typed" t
-	      end
-	  end
-	| _ => idtac tac_sound "is not a soudness theorem."
-  end.
-
