MirrorCharge!/src/MirrorCharge/Java/SymEx.v
@@ -221,7 +221,7 @@ Definition fieldLookupTac : rtac typ (expr typ func) :=
 		  	match class_lookup C P with
     	      | Some Class =>
     	        match @exprUnify (ctx_subst c) typ func _ _ _ _ _ 3
-                                 tus tvs 0 s f (mkFields (c_fields Class)) tyVarList with
+                                 tus tvs 0 f (mkFields (c_fields Class)) tyVarList s with
                   | Some s => Solved s
                   | None   => Fail
                 end
@@ -234,7 +234,7 @@ Definition FIELD_LOOKUP := fieldLookupTac.
 
 Require Import MirrorCharge.ModularFunc.ListFunc.
 
-	Definition foldTac (e : expr typ func) (args : list (expr typ func))
+	Definition foldTac (l : list (option (expr typ func))) (e : expr typ func) (args : list (expr typ func))
 	: expr typ func :=
 	  match listS e with
 	    | Some (pFold t u) =>
@@ -246,7 +246,7 @@ Require Import MirrorCharge.ModularFunc.ListFunc.
 	    | _ => apps e args
 	  end.
 
-Definition FOLD := SIMPLIFY (typ := typ) (fun _ _ _ _ => beta_all foldTac nil nil).
+Definition FOLD := SIMPLIFY (typ := typ) (fun _ _ _ _ => beta_all foldTac).
 
 Require Import ExtLib.Tactics.Consider.
 Require Import ExtLib.Tactics.
@@ -257,21 +257,36 @@ Proof.
   apply SIMPLIFY_sound.
   intros; simpl.
   forward.
+  rewrite <- H.
+  Check beta_all_sound.
   (* beta_all_sound is missing *)
   admit.
 Qed.
-
-Definition BETA := SIMPLIFY (typ := typ) (fun _ _ _ _ => beta_all (@apps typ func) nil nil).
+Check apps.
+Definition BETA := SIMPLIFY (typ := typ) (fun _ _ _ _ => beta_all (fun _ => @apps typ func)).
 
 Lemma BETA_sound : rtac_sound BETA.
 Proof.
   unfold BETA.
   apply SIMPLIFY_sound.
   intros; simpl; forward.
+  (*
+  SearchAbout full_reducer.
+  assert (full_reducer_ok (fun _ => apps (sym := func))). {
+    clear.
+    intros e vars tus tvs tus' tvs' P Hvars es t targs Hexpr.
+  }
+  unfold full_reducer_ok.
+  
+  Print full_reducer.
+  pose proof (beta_all_sound).
+  SearchAbout beta_all.
+  rewrite <- H.*)
   admit.
 Qed.
 
-Definition THEN (r1 r2 : rtac typ (expr typ func)) := THEN r1 (runOnGoals r2).
+Definition THEN (r1 r2 : rtac typ (expr typ func)) := 
+  THEN (THEN (THEN (INSTANTIATE typ func) (runOnGoals r1)) (runOnGoals (INSTANTIATE typ func))) (runOnGoals r2).
 
 Definition EQSUBST := THEN (THEN (APPLY typ func eq_to_subst_lemma) 
 	(INSTANTIATE typ func)) (SUBST typ func).
@@ -355,26 +370,40 @@ Definition solve_alloc rw : rtac typ (expr typ func) :=
                         FIELD_LOOKUP ::
                         THEN FOLD (solve_entailment rw) :: nil)).
 
+Require Import MirrorCore.RTac.Minify.
+Check MINIFY.
+Print rtacK.
+Check runOnGoals (SUBST typ func).
+Check THENK.
+Print rtacK.
+Definition THEN' := @MirrorCore.RTac.Then.THEN typ (expr typ func).
 
 Definition simStep (rw : rewriter (typ := typ) (func := func)) (r : rtac typ (expr typ func)) :=
-    THEN (THEN (THEN (THEN (THEN (INSTANTIATE typ func) (SUBST typ func))
+    THEN (THEN' IDTAC (@MINIFY typ (expr typ func) _)) r.
+    (*
+    THEN (THEN (THEN (THEN (THENK (@MINIFY typ func _) (@runOnGoals typ (expr typ func) _ (SUBST typ func)))
     	(TRY PULL_TRIPLE_EXISTS)) (STEP_REWRITE rw)) (REPEAT 10 PULL_TRIPLE_EXISTS)) r.
-
+*)
 Set Printing Depth 100.
-
-Print alloc_lemma.
-
-Print runOnGoals.
-
+Check MirrorCore.RTac.ThenK.THENK.
+Check FIRST.
 Fixpoint tripleE (c : cmd) rw : rtac typ (expr typ func) :=
 	match c with
-	    | cskip => simStep rw (THEN (APPLY typ func skip_lemma) 
-	                 (solve_entailment rw))
+	    | cskip => simStep rw (THEN' (APPLY typ func skip_lemma) 
+	                 (THENK (@MINIFY typ (expr typ func) _)
+	                   (THENK (runOnGoals (solve_entailment rw))
+	                      (@MINIFY typ (expr typ func) _))))
 	    | calloc x C => simStep rw (THEN (EAPPLY typ func (alloc_lemma x C)) 
 	    	(FIRST (solve_alloc rw :: solve_entailment rw :: nil)))
 		| cseq c1 c2 => simStep rw (THEN (EAPPLY typ func (seq_lemma c1 c2))
-						              (FIRST ((fun x => tripleE c1 rw x)::(fun x => tripleE c2 rw x)::nil)))
-		| cassign x e => simStep rw (THEN (EAPPLY typ func (assign_lemma x e)) (solve_entailment rw))
+						              
+						                (FIRST ((fun x => tripleE c1 rw x)::(fun x => tripleE c2 rw x)::nil)))
+						                
+(*		| cseq c1 c2 => simStep rw (THEN' (EAPPLY typ func (seq_lemma c1 c2))
+						              (THENK (@MINIFY typ (expr typ func) _) 
+						                (THENK (runOnGoals (FIRST ((fun x => tripleE c1 rw x)::(fun x => tripleE c2 rw x)::nil))
+						                ) (@MINIFY typ (expr typ func) _))))
+*)		| cassign x e => simStep rw (THEN (EAPPLY typ func (assign_lemma x e)) (solve_entailment rw))
 		| cread x y f => simStep rw (THEN (EAPPLY typ func (read_lemma x y f)) (solve_entailment rw))
 		| cwrite x f e => simStep rw (THEN (EAPPLY typ func (write_lemma x f e)) (solve_entailment rw))
 		| _ => IDTAC
@@ -404,22 +433,22 @@ Qed.
 
 Definition mkPointsto (x : expr typ func) (f : field) (e : expr typ func) : expr typ func :=
    mkAp tyVal tyAsn 
-        (mkAp tyField (tyArr tyVal tyAsn)
-              (mkAp tyVal (tyArr tyField (tyArr tyVal tyAsn))
-                    (mkConst (tyArr tyVal (tyArr tyField (tyArr tyVal tyAsn))) 
+        (mkAp tyString (tyArr tyVal tyAsn)
+              (mkAp tyVal (tyArr tyString (tyArr tyVal tyAsn))
+                    (mkConst (tyArr tyVal (tyArr tyString (tyArr tyVal tyAsn))) 
                              fPointsto)
                     x)
-              (mkConst tyField (mkField f)))
+              (mkConst tyString (mkField f)))
         e.
         
 Definition mkPointstoVar x f e : expr typ func :=
    mkAp tyVal tyAsn 
-        (mkAp tyField (tyArr tyVal tyAsn)
-              (mkAp tyVal (tyArr tyField (tyArr tyVal tyAsn))
-                    (mkConst (tyArr tyVal (tyArr tyField (tyArr tyVal tyAsn))) 
+        (mkAp tyString (tyArr tyVal tyAsn)
+              (mkAp tyVal (tyArr tyString (tyArr tyVal tyAsn))
+                    (mkConst (tyArr tyVal (tyArr tyString (tyArr tyVal tyAsn))) 
                              fPointsto)
                     (App fStackGet (mkVar x)))
-              (mkConst tyField (mkField f)))
+              (mkConst tyString (mkField f)))
         e.
         
 Require Import Java.Semantics.OperationalSemantics.
@@ -444,8 +473,22 @@ Fixpoint seq_skip n :=
 Ltac solve_equation :=
 	intros; repeat ((repeat eexists); try reflexivity).
 	
-Ltac cbv_denote e :=
-          eval cbv [
+Definition goalD_Prop (uvar_env var_env : env) goal :=
+  let (tus, us) := split_env uvar_env in
+  let (tvs, vs) := split_env var_env in
+  match goalD tus tvs goal with
+    | Some e => e us vs
+    | None => False
+  end.
+  
+Definition exprD_Prop (uvar_env var_env : env) e :=
+  match exprD uvar_env var_env e tyProp with
+    | Some e' => e' 
+    | None => True
+  end.
+(*
+Ltac cbv_denote :=
+          cbv [
           goalD_aux
           
 		  (* ExprD' *)
@@ -472,7 +515,7 @@ Ltac cbv_denote e :=
           
           TypesI.typD 
           typ2_match typ2 typ2_cast
-          typ0_match typ0 typ0_cast
+          typ0_match typ0 typ0_cast SubstTypeD_typ
           (* ExprI *)
           
           MirrorCore.VariablesI.Var ExprVariables.ExprVar_expr
@@ -630,13 +673,8 @@ Ltac cbv_denote e :=
           JavaFunc.mkTriple JavaFunc.mkFieldLookup JavaFunc.mkTypeOf
           JavaFunc.mkProgEq JavaFunc.mkExprList JavaFunc.evalDExpr
           
-          (* Applicative *)
-  (*        
-          ExtLib.Structures.Applicative.ap ExtLib.Structures.Applicative.pure
- 	      Applicative_Fun
-          
-          Charge.Logics.Pure.pure
-    *)      
+(* OTHER *)
+  
           SubstType_typ
           
           goalD propD exprD'_typ0 exprD split_env
@@ -657,7 +695,57 @@ Ltac cbv_denote e :=
           HList.hlist_app
           Quant._foralls
           Quant._exists
-          ] in e.
+          goalD_Prop
+          ].
+
+Lemma run_rtac_More tac s goal e
+  (Hsound : rtac_sound tac) 
+  (Hres : run_tac tac (GGoal e) = More_ s goal) :
+  goalD_Prop nil nil goal -> exprD_Prop nil nil e.
+Proof.
+  intros He'.
+  apply runOnGoals_sound_ind with (g := GGoal e) (ctx := CTop nil nil) 
+  	(s0 := TopSubst (expr typ func) nil nil) in Hsound.
+  unfold rtac_spec in Hsound. simpl in Hsound.
+  unfold run_tac in Hres. simpl in Hres.
+  rewrite Hres in Hsound.
+  assert (WellFormed_Goal nil nil (GGoal (typ := typ) e)) as H1 by constructor.
+  assert (WellFormed_ctx_subst (TopSubst (expr typ func) nil (@nil typ))) as H2 by constructor.
+  specialize (Hsound H1 H2).
+  destruct Hsound as [Hwfs [Hwfg Hsound]].
+  unfold propD, exprD'_typ0 in Hsound.
+  simpl in Hsound. unfold exprD_Prop, exprD; simpl.
+  forward; inv_all; subst.
+
+  destruct Hsound.
+  inversion Hwfs; subst.
+  simpl in H0; inv_all; subst.
+  unfold pctxD in H0; inv_all; subst.
+  apply H5.
+  unfold goalD_Prop in He'. simpl in He'. forward; inv_all; subst.
+Qed.
+
+Lemma run_rtac_Solved tac s e
+  (Hsound : rtac_sound tac) 
+  (Hres : run_tac tac (GGoal e) = Solved s) :
+  exprD_Prop nil nil e.
+Proof.
+  unfold run_tac in Hres.
+  unfold rtac_sound in Hsound.
+  assert (WellFormed_Goal nil nil (GGoal (typ := typ) e)) as H1 by constructor.
+  assert (WellFormed_ctx_subst (TopSubst (expr typ func) nil (@nil typ))) as H2 by constructor.
+  specialize (Hsound _ _ _ _ Hres H1 H2).
+  destruct Hsound as [Hwfs Hsound].
+  simpl in Hsound.
+  unfold propD, exprD'_typ0 in Hsound.
+  unfold exprD_Prop.
+  
+  simpl in Hsound. unfold exprD. simpl. forward.
+  destruct Hsound. 
+  SearchAbout pctxD.
+  inversion Hwfs; subst. simpl in H8. inv_all; subst.
+  admit.
+Qed.
 
 Ltac run_rtac tac_sound :=
   match type of tac_sound with
@@ -670,32 +758,21 @@ Ltac run_rtac tac_sound :=
 	      let goal := eval unfold name in name in
 	      match t with
 	        | Some ?t =>
-	          let goal_result := constr:(run_tac tac (GGoal goal)) in 
-	          let result := eval vm_compute in goal_result in 
+	          let goal_result := constr:(run_tac tac (GGoal name)) in 
+	          let result := eval vm_compute in goal_result in
 	          match result with
-	            | More_ ?s ?g =>
-	              let Q := cbv_denote (goalD_aux nil nil g Hnil Hnil) in
-	              match Q with
-	                | Some ?Q' => 
-	                  cut Q'; [
-		              let P := cbv_denote (exprD nil nil goal tyProp) in 
-		              pose (H1 := @eq_refl (option Prop) P <: 
-		              	exprD nil nil goal tyProp = P);
-		              pose (H2 := @eq_refl (Result (CTop nil nil)) result <: 
-		              	run_tac tac (GGoal goal) = result)  ;
-		              pose (H3 := @eq_refl (option Prop) Q <:
-		              	goalD_aux nil nil g Hnil Hnil = Q);
-		              exact (@run_rtac_More tac _ _ _ _ _ H1 H2 H3 tac_sound)|]
-		            | None => idtac "Unable to find a denotation for" Q
-		          end
+	            | More_ ?s ?g => 
+	              cut (goalD_Prop nil nil g); [
+	                let goal_resultV := g in
+	               (* change (goalD_Prop nil nil goal_resultV -> exprD_Prop nil nil name);*)
+	                exact_no_check (@run_rtac_More tac _ _ _ tac_sound
+	                	(@eq_refl (Result (CTop nil nil)) (More_ s goal_resultV) <:
+	                	   run_tac tac (GGoal goal) = (More_ s goal_resultV)))
+	                | cbv_denote
+	              ]
 	            | Solved ?s =>
-	              let P := cbv_denote (exprD nil nil goal tyProp) in
-	              let H1 := fresh "H" in
-	              pose (H1 := @eq_refl (option Prop) P <:
-	                exprD nil nil goal tyProp = P);
-		          pose (H2 := @eq_refl (Result (CTop nil nil)) result <: 
-		            run_tac tac (GGoal goal) = result);
-	              exact (@run_rtac_Solved tac _ _ _ H1 H2 tac_sound)
+	              exact_no_check (@run_rtac_Solved tac s name tac_sound 
+	                (@eq_refl (Result (CTop nil nil)) (Solved s) <: run_tac tac (GGoal goal) = Solved s))
 	            | Fail => idtac "Tactic" tac "failed."
 	            | _ => idtac "Error: run_rtac could not resolve the result from the tactic :" tac
 	          end
@@ -704,32 +781,126 @@ Ltac run_rtac tac_sound :=
 	  end
 	| _ => idtac tac_sound "is not a soudness theorem."
   end.
+*)
+Require Import ExtLib.Structures.Applicative.
+Local Instance Applicative_Fun A : Applicative (Fun A) :=
+{ pure := fun _ x _ => x
+; ap := fun _ _ f x y => (f y) (x y)
+}.
 
 Definition testSkip n : Prop :=
   forall (G : spec) (P : sasn), G |-- triple P P (seq_skip n).
 
+Require Import MirrorCharge.RTac.Tactics.
 
-Lemma test_skip_lemma3 : testSkip 20.
+Lemma test_skip_lemma3 : testSkip 0.
 Proof.
+  idtac "start".
   unfold testSkip; simpl.
-  Time run_rtac (@runTac_sound rw_fail).
-  solve_equation.
+  Time run_rtac reify_imp term_table (@runTac_sound rw_fail).
+  Print THEN.
+  intros.
+  eexists. eexists. eexists. eexists.
 Time Qed.
 
 Definition test_alloc : expr typ func :=
 	mkEntails tySpec (mkProgEq (mkProg ListProg))
 		(mkTriple (mkTrue tySasn) (mkCmd (cseq (calloc "x" "NodeC") cskip)) (mkFalse tySasn)).
 
-
+Require Import Charge.Logics.BILogic.
   
   Lemma test_alloc_correct : 
-  prog_eq ListProg |-- triple ltrue lfalse ((calloc "x" "NodeC");;Skip).
+  prog_eq ListProg |-- triple empSP lfalse ((calloc "x" "NodeC");;Skip).
 Proof.
-
   Time run_rtac (@runTac_sound rw_fail).
-
+  simpl.
+(*
+  eexists.
+  eexists.
+  eexists.
+  eexists.
+  
+  split.
+  split.
+  split.
+  split.
+  reflexivity.
+  split.
+  reflexivity.
+  split.
+  reflexivity.
+  apply I.
+  eexists.  
+  eexists.
+  eexists.
+  eexists.
+  eexists.
+  eexists.
+  split.
+  split.
+  split.
+  split.
+  split.
+  split.
+  split.
+  split.
+  split.
+  split.
+  split.
+  split.
+  split.
+  eexists.
+  eexists.
+  eexists.
+  eexists.
+  split.
+  split.
+  split.
+  split.
+  split.
+  split.
+  split.
+  split.
+  split.
+  split.
+  intros.
+  eexists.
+  eexists.
+  eexists.
+  split.
+  split.
+  split.
+  split.
+  split.
+  split.
+  split.
+  split.
+  eexists.
+  eexists.
+  eexists.
+  eexists.
+  split.
+  split.
+  split.
+  split.
+  split.
+  split.
+  split.
+  split.
+  split.
+  split.
+  reflexivity.
+   eexists. 
+  split.
+  eexists.
+  do 3 eexists.
+  solve_equation.
+*)
+admit.
+Qed.
+(*
 Eval vm_compute in runTac test_alloc rw_fail.
-
+*)
 Definition runTac2 (tac : expr typ func) rw := 
    (THEN (THEN (THEN (THEN (REPEAT 1000 (INTRO typ func)) (symE rw)) 
 	(INSTANTIATE typ func)) BETA) (CANCELLATION typ func tySasn is_pure))
@@ -746,98 +917,100 @@ Eval vm_compute in (CANCELLATION typ func tySasn is_pure) nil nil 0 0 (CTop nil 
   (mkEntails tySasn (mkTrue tySasn) (mkTrue tySasn)).
   
 
-
+(*
 Definition test_read2 :=
   	(mkEntails tySpec (mkTrue tySpec)
   	           (mkTriple (mkPointstoVar "o" "f" (mkConst tyVal (mkVal (vint 3))))
   	                     (mkCmd (cseq (cread "x" "o" "f") cskip))
   	                     (mkPointstoVar "o" "f" (mkConst tyVal (mkVal (vint 3)))))).
-Time Eval vm_compute in runTac test_read rw_fail.
-Check instantiate.
+*)  	                     
 
-Time Eval vm_compute in runTac test_read2 rw_fail.
-
+Check ExtLib.Structures.Applicative.pure.
 
 
+Lemma test_read2 : ltrue |-- 
+    triple 
+      (ap_pointsto [("o": var), ("f" : field), pure (T := Fun (Lang.stack)) (vint 3)] ** 
+       ap_pointsto [("o": var), ("g" : field), pure (T := Fun (Lang.stack)) (vint 4)]) 
+      (ap_pointsto [("o": var), ("f": field), pure (T := Fun (Lang.stack)) (vint 3)] ** 
+      (ap_pointsto [("o": var), ("g": field), pure (T := Fun (Lang.stack)) (vint 4)]))
+      (cseq (cread "x" "o" "f") (cseq (cread "y" "o" "g") cskip)).                    
+Proof.
+  Time run_rtac (@runTac_sound rw_fail).
+Qed.
 
-
-Definition test_write :=
-  	(mkEntails tySpec (mkTrue tySpec)
-  	           (mkTriple (mkPointstoVar "o" "f" (mkConst tyVal (mkVal (vint 3))))
-  	                     (mkCmd (cwrite "o" "f" (E_val (vint 4))))
-  	                     (mkPointstoVar "o" "f" (mkConst tyVal (mkVal (vint 4)))))).
-
-Time Eval vm_compute in runTac test_write rw_fail.
-
-Definition testSwap :=
-	mkForall tyVal tyProp
-		(mkForall tyVal tyProp
-		  	(mkEntails tySpec (mkTrue tySpec)
-		  	           (mkTriple (mkStar tySasn (mkStar tySasn 
-		  	           			    (mkPointstoVar "o" "f1" (mkConst tyVal (Var 1)))
-		  	           			    (mkPointstoVar "o" "f0" (mkConst tyVal (Var 0)))) (mkEmp tySasn))
-		  	           			 (mkCmd (cseq (cread "x0" "o" "f0")
-  	                                          (cseq (cread "x1" "o" "f1")
-  	                                                (cseq (cwrite "o" "f1" (E_var "x0"))
-  	                                                      (cseq (cwrite "o" "f0" (E_var "x1")) cskip)))))
-		  	           			 (mkStar tySasn (mkStar tySasn 
-		  	           			    (mkPointstoVar "o" "f1" (mkConst tyVal (Var 0)))
-		  	           			    (mkPointstoVar "o" "f0" (mkConst tyVal (Var 1)))) (mkEmp tySasn))))).
-SearchAbout string nat.
-
-Fixpoint mkPre n :=
+Lemma test_write :
+	ltrue |--
+	triple
+      (ap_pointsto [("o": var), ("f" : field), pure (T := Fun (Lang.stack)) (vint 3)]) 
+      (ap_pointsto [("o": var), ("f": field), pure (T := Fun (Lang.stack)) (vint 4)])
+      (cseq (cwrite "o" "f" (E_val (vint 4))) cskip).                    
+Proof.
+  Time run_rtac (@runTac_sound rw_fail).
+Qed.
+*)
+Require Import Charge.Logics.BILogic.
+Require Import BinInt.
+SearchAbout nat Z.
+Fixpoint mkSwapPre n : sasn :=
 	match n with
-	  | 0   => mkEmp tySasn
-	  | S n => mkStar tySasn (mkPointstoVar "o" (append "f" (nat2string10 n)) (mkConst tyVal (Var n)))
-	                         (mkPre n)
-	end.
+	  | 0   => empSP
+	  | S n => ap_pointsto [("o": var), (append "f" (nat2string10 n) : field), 
+	  	                     (eval (E_val (vint (Z.of_nat n))))] **
+	           mkSwapPre n
+	end.  
+
 	
-Fixpoint mkPostAux n m :=
+Fixpoint mkSwapPostAux n m :=
   match n with
-    | 0 => mkEmp tySasn
-    | S n => mkStar tySasn (mkPointstoVar "o" (append "f" (nat2string10 n)) (mkConst tyVal (Var (m - (S n)))))
-                           (mkPostAux n m)
-  end.
+    | 0 => empSP
+	| S n => ap_pointsto [("o": var), (append "f" (nat2string10 n) : field), 
+	  	                     (eval (E_val (vint (Z.of_nat (m - (S n))))))] **
+	         mkSwapPostAux n m
+  end.           
   
-Definition mkPost n := mkPostAux n n.
+Definition mkSwapPost n := mkSwapPostAux n n.
 
 Fixpoint mkRead n c :=
 	match n with
 	  | 0 => c
-	  | S n => cseq (cread (append "x" (nat2string10 n)) "o" (append "f" (nat2string10 n)))
+	  | S n => cseq (cread ((append "x" (nat2string10 n):var)) ("o":var) ((append "f" (nat2string10 n)):field))
 	                (mkRead n c)
     end.
 						
 Fixpoint mkWriteAux n m c :=
 	match n with
 	  | 0 => c
-	  | S n => cseq (cwrite "o" (append "f" (nat2string10 n)) (E_var (append "x" (nat2string10 (m - (S n))))))
+	  | S n => cseq (cwrite ("o":var) (append "f" (nat2string10 n)) (E_var (append "x" (nat2string10 (m - (S n))))))
 	                (mkWriteAux n m c)
     end.
 
 Definition mkWrite n c := mkWriteAux n n c.
 
-Fixpoint mkSwapAux n P c Q :=
-	match n with
-	  | 0 => (mkEntails tySpec (mkTrue tySpec) (mkTriple P c Q))
-	  | S n => mkForall tyVal tyProp (mkSwapAux n P c Q)
-	end.
-
-Definition mkSwapProg n c := mkRead n (mkWrite n c).
+Definition mkSwapProg (n : nat) (c : cmd) := mkRead n (*(mkWrite n c) *) c.
 	
 Definition mkSwap n :=
-	mkSwapAux n (mkPre n) (mkCmd (mkSwapProg n cskip)) (mkPost n).
+	ltrue |-- triple (mkSwapPre n) (mkSwapPost n) (mkSwapProg n cskip).
 
-Definition mkSwapFalse n :=
-	mkSwapAux n (mkPre n) (mkCmd (mkSwapProg n cskip))(* (mkFalse tySasn).*).
-
-Time Eval vm_compute in (mkCmd (mkSwapProg 2 (mkSwapProg 2 cskip))).
-
-
-Definition mkSwap2 n :=
-	mkSwapAux n (mkPre n) (mkCmd (mkSwapProg n (mkSwapProg n cskip)))(* (mkPre n).*).
-Eval vm_compute in mkSwap 5.
-Check EAPPLY.
+Lemma test_swap : mkSwap 1.
+Proof.
+  Opaque ap.
+  unfold mkSwap, mkSwapPre, mkSwapPost, mkSwapProg, mkSwapPostAux, mkRead, mkWrite, mkWriteAux.
+  run_rtac (@runTac_sound rw_fail).
+  repeat eexists.
+  reflexivity.
+  reflexivity.
+  admit.
+Qed.
+  cbv [SubstTypeD_typ].
+  simpl.
+  assert (("o" : String.string) = "o").
+  simpl.
+  cbv [mkRead mkWrite mkWriteAux app nat2string10 nat2string Wf.Fix_sub Wf.Fix_F_sub NPeano.ltb NPeano.leb
+       Char.digit2ascii ascii_of_nat nat_of_ascii BinNat.N.of_nat BinNat.N.to_nat N_of_ascii ascii_of_N
+       N_of_digits BinNat.N.add BinNat.N.mul].
+  run
+  
 Time Eval vm_compute in runTac (mkSwap 4) rw_fail.
 
 Time Eval vm_compute in 
